reify/reverse_reify.v
@@ -4,86 +4,17 @@ Require Import functions.
 Require Import progs.reverse.
 Require Import progs.list_dt.
 Require Import sep.
+Require Import wrapExpr.
 Local Open Scope logic.
 
+
+(*Some definitions needed from the example file (verif_reverse.v) *)
 Instance LS: listspec t_struct_list _tail.
 Proof. eapply mk_listspec; reflexivity. Defined.
 
 Definition sum_int := fold_right Int.add Int.zero.
 
-
-(*types we need that aren't defined yet... 
-this is just an example, we don't really need this one*)
-Definition LS_type := cons (no_eqb_type (listspec t_struct_list _tail)) nil.
-
-Module uk_types <: unknown_types.
-Definition unknown_types := LS_type.
-End uk_types.
-
-Module funcs := funcs uk_types.
-Import funcs.
-Import all_types.
-
-Definition list_spec_tv := Expr.tvType (length our_types).
-Compute (elemtype LS).
-
-
-(*Separation logic predicate just for this file *)
-Definition lseg_signature :=
-Sep.PSig all_types (cons share_tv
-                   (cons list_int_tv (cons val_tv (cons val_tv nil))))
-(lseg LS).
-
-Definition predicates := lseg_signature :: nil.
-Check predicates.
-Definition lseg_p := length sep_predicates.
-
-(*Functions just for this file. These three represent variables
-  that are above the line. *)
-Definition more_funcs rho contents sh :=
-make_environ_signature rho ::
-make_list_int_signature contents ::
-make_share_signature sh :: nil.
-
-Definition rho_fv := length functions.
-Definition contents_fv := S rho_fv.
-Definition sh_fv := S contents_fv.
-
-Definition rho_f := nullary_func rho_fv.
-Definition contents_f := nullary_func contents_fv.
-Definition sh_f := nullary_func sh_fv.
-
-(*Some constants we will use *)
-
-Definition true_c := prop_const True.
-Definition zero_c := val_const (Vint (Int.repr 0)).
-Definition _p_c := id_const _p.
-Definition _t_c := id_const _t.
-Definition _s_c := id_const _s.
-Definition nullval_c := val_const nullval.
-
-
-(*Put it together with functions and stars *)
-Definition eval_id_p := eval_id_func _p_c rho_f.
-Definition eval_id_t := eval_id_func _t_c rho_f.
-Definition eval_id_s := eval_id_func _s_c rho_f.
-Definition eq1 := val_eq eval_id_t eval_id_p.
-Definition eq2 := val_eq eval_id_s zero_c.
-
-
-Definition pure := and_func eq1 (and_func eq2 true_c).
-Definition our_inj e := Sep.Star (Sep.Inj e) (Sep.Emp all_types).
-Definition TT_s := our_inj true_c.
-
-Definition lseg_func := @Sep.Func all_types lseg_p
-(sh_f :: contents_f :: eval_id_p :: nullval_c :: nil).
-
-Definition left_side :=
-Sep.Star TT_s 
-(Sep.Star (our_inj pure)
-(Sep.Star lseg_func (Sep.Emp all_types))).
-
-Definition Delta :=
+Definition Delta := 
 (PTree.Node
          (PTree.Node
             (PTree.Node
@@ -156,7 +87,7 @@ Definition Delta :=
                               (WITH x : share * list int PRE 
                                [(_p, tptr t_struct_list)]
                                (let (sh0, contents0) := x in
-                                `(lseg LS sh0 contents0) 
+                                `(lseg LS sh0 (map Vint contents0))
                                   (eval_id _p) `nullval) POST  [tint]
                                (let (_, contents0) := x in
                                 local
@@ -176,7 +107,7 @@ Definition Delta :=
                         (Some
                            (Global_func
                               (WITH  sh0 : share, contents0 : 
-                               list int PRE  [(_p, tptr t_struct_list)]
+                               list val PRE  [(_p, tptr t_struct_list)]
                                (fun x0 : environ =>
                                 !!writable_share sh0 &&
                                 `(lseg LS sh0 contents0) 
@@ -220,8 +151,8 @@ Definition Delta :=
                             (WITH x : share * list int PRE 
                              [(_p, tptr t_struct_list)]
                              (let (sh0, contents0) := x in
-                              `(lseg LS sh0 contents0) (eval_id _p) `nullval)
-                             POST  [tint]
+                              `(lseg LS sh0 (map Vint contents0))
+                                (eval_id _p) `nullval) POST  [tint]
                              (let (_, contents0) := x in
                               local (`(eq (Vint (sum_int contents0))) retval)))))
                       PTree.Leaf) None PTree.Leaf) None PTree.Leaf)) None
@@ -239,7 +170,7 @@ Definition Delta :=
                       (Some
                          (Global_func
                             (WITH  sh0 : share, contents0 : 
-                             list int PRE  [(_p, tptr t_struct_list)]
+                             list val PRE  [(_p, tptr t_struct_list)]
                              (fun x0 : environ =>
                               !!writable_share sh0 &&
                               `(lseg LS sh0 contents0) 
@@ -281,8 +212,8 @@ Definition Delta :=
                           (WITH x : share * list int PRE 
                            [(_p, tptr t_struct_list)]
                            (let (sh0, contents0) := x in
-                            `(lseg LS sh0 contents0) (eval_id _p) `nullval)
-                           POST  [tint]
+                            `(lseg LS sh0 (map Vint contents0)) 
+                              (eval_id _p) `nullval) POST  [tint]
                            (let (_, contents0) := x in
                             local (`(eq (Vint (sum_int contents0))) retval)))))
                     PTree.Leaf) None PTree.Leaf) None PTree.Leaf)) None
@@ -300,7 +231,7 @@ Definition Delta :=
                     (Some
                        (Global_func
                           (WITH  sh0 : share, contents0 : 
-                           list int PRE  [(_p, tptr t_struct_list)]
+                           list val PRE  [(_p, tptr t_struct_list)]
                            (fun x0 : environ =>
                             !!writable_share sh0 &&
                             `(lseg LS sh0 contents0) (eval_id _p) `nullval x0)
@@ -322,6 +253,157 @@ Definition Delta :=
                           (WITH u : unit PRE  []main_pre prog u POST  [tint]
                            main_post prog u))) PTree.Leaf) None PTree.Leaf)))).
 
+
+(*types we need that aren't defined yet... 
+this is just an example, we don't really need this one*)
+Definition LS_type := cons (no_eqb_type (listspec t_struct_list _tail)) nil.
+
+Module uk_types <: unknown_types.
+Definition unknown_types := LS_type.
+End uk_types.
+
+Module funcs := funcs uk_types.
+Import funcs.
+Import all_types.
+
+Definition list_spec_tv := Expr.tvType (length our_types).
+
+
+(*Separation logic predicate just for this file *)
+
+Definition lseg_signature :=
+Sep.PSig all_types (cons share_tv
+                   (cons list_val_tv (cons val_tv (cons val_tv nil))))
+(lseg LS).
+
+Definition predicates := lseg_signature :: nil.
+Definition lseg_p := length sep_predicates.
+
+(*Functions just for this file. These three represent variables
+  that are above the line. *)
+
+Definition sum_int_signature :=
+Expr.Sig all_types (list_int_tv :: nil)
+int_tv sum_int.
+
+
+Definition more_funcs rho contents sh :=
+make_environ_signature rho ::
+make_list_int_signature contents ::
+make_share_signature sh ::
+sum_int_signature :: nil.
+
+
+Definition rho_f := length functions.
+Definition contents_f := S rho_f.
+Definition sh_f := S contents_f.
+Definition sum_int_f := S sh_f.
+
+Definition rho_func := nullary_func rho_f.
+Definition contents_func := nullary_func contents_f.
+Definition sh_func := nullary_func sh_f.
+Definition sum_int_func i1  := 
+@Expr.Func all_types sum_int_f (i1  :: nil).
+
+(*Some constants we will use *)
+
+Definition true_c := prop_const True.
+Definition zero_c := val_const (Vint (Int.repr 0)).
+Definition _p_c := id_const _p.
+Definition _t_c := id_const _t.
+Definition _s_c := id_const _s.
+Definition nullval_c := val_const nullval.
+Definition delta_c := tycontext_const Delta.
+
+(*Put it together with functions and stars *)
+Definition eval_id_p := eval_id_func _p_c rho_func.
+Definition eval_id_t := eval_id_func _t_c rho_func.
+Definition eval_id_s := eval_id_func _s_c rho_func.
+Definition eq1 := val_eq eval_id_t eval_id_p.
+Definition eq2 := val_eq eval_id_s zero_c.
+
+
+Definition pure := and_func true_c (and_func eq1 (and_func eq2 true_c)).
+
+Definition lseg_func := @Sep.Func all_types lseg_p
+(sh_func :: (map_vint_func contents_func) :: eval_id_p :: nullval_c :: nil).
+
+Definition left_side :=
+(Sep.Star (Sep.Inj pure)
+(Sep.Star lseg_func (Sep.Emp all_types))).
+
+Definition sum_int_contents :=
+sum_int_func (contents_func).
+
+Definition sub_val := 
+vint_func (int_sub_func sum_int_contents sum_int_contents).
+
+Definition eq_s_sub :=
+val_eq sub_val eval_id_s.
+
+Definition pure_r :=
+and_func true_c (and_func eq_s_sub true_c).
+
+Definition lseg_r := 
+@Sep.Func all_types lseg_p (sh_func :: (map_vint_func contents_func) :: eval_id_t :: nullval_c :: nil).
+ 
+Definition sep_r := Sep.Star (Sep.Star (Sep.Const all_types (!!True)) lseg_r) (Sep.Emp all_types).
+
+Definition right_side := 
+Sep.Star (Sep.Inj pure_r)
+sep_r.
+
+Definition tc_environ_r := 
+tc_environ_func delta_c rho_func.
+
+
+Ltac unfold_VericSepLogic := simpl; unfold VericSepLogic.star, 
+VericSepLogic.inj, VericSepLogic.emp.
+
+Lemma convert_inj : forall S Q, !!S && Q  = (!!S && emp) * Q.
+intros.
+apply pred_ext.
+ entailer!. 
+entailer!.
+Qed.
+
+(*When prepare_reify is finished, all !!s should be in the form
+!!P && emp * ... so that they can be converted to SepExpr.Inj 
+this tactic is likely incomplete*)
+Ltac prepare_reify :=
+autorewrite with gather_prop;
+match goal with 
+| [ |- !!?X && _ |-- !!?Y && _] => rewrite (convert_inj X); rewrite (convert_inj Y)
+| [ |- !!?X && _ |-- _] => rewrite (convert_inj X)
+end.
+
+(*Turns a reified derives into a reified goal with no assumptions, 
+sort of a base case for rev_reify *)
+Ltac start_goalD :=
+match goal with 
+[ |- derivesD ?t ?f ?p ?e ?v ?d] => 
+replace (derivesD t f p e v d) with (goalD t f p e v (nil, d)) by reflexivity
+end.
+
+(*Pulls down any reified assumptions and puts them into 
+a goal *)
+Ltac rev_reify :=
+repeat match goal with
+| [ H : force_Opt (Expr.exprD ?f ?e ?v ?P ?ty) False |- goalD ?t ?f ?p ?e ?v (?l, ?d) ] => revert H; 
+replace (force_Opt (Expr.exprD f e v P ty) False ->
+goalD t f p e v (l, d)) with
+(goalD t f p e v (P::l, d)) by reflexivity
+end.
+
+Ltac finish_reify :=
+match goal with 
+[ |- @Sep.sexprD ?t ?f ?p ?e ?v ?le |-- Sep.sexprD ?f ?p ?e ?v ?re ] => 
+  replace (Sep.sexprD f p e v le |-- Sep.sexprD f p e v re) with 
+  (derivesD t f p e v (le, re)) by reflexivity end;
+start_goalD;
+rev_reify.
+
+
 Lemma while_entail1 :
   name _t ->
   name _p ->
@@ -332,28 +414,41 @@ Lemma while_entail1 :
    LOCAL 
    (tc_environ
       Delta;
-   `eq (eval_id _t) (eval_expr (Etempvar _p (tptr t_struct_list)));
+   `eq (eval_id _t) (eval_expr (Etempvar _p (tptr t_struct_list))
+);
    `eq (eval_id _s) (eval_expr (Econst_int (Int.repr 0) tint)))
-   SEP  (`(lseg LS sh contents) (eval_id _p) `nullval)
+   SEP  (`(lseg LS sh (map Vint contents)) (eval_id _p) `nullval)
    |-- PROP  ()
        LOCAL 
        (`(eq (Vint (Int.sub (sum_int contents) (sum_int contents))))
           (eval_id _s))
-       SEP  (TT; `(lseg LS sh contents) (eval_id _t) `nullval).
+       SEP  (TT; `(lseg LS sh (map Vint contents)) (eval_id _t) `nullval).
 Proof.
 intros.
 go_lower0.
-assert 
-(( !!True &&
-   (!!(eval_id _t rho = eval_id _p rho /\
-       eval_id _s rho = Vint (Int.repr 0) /\ True) &&
-    (lseg LS sh contents (eval_id _p rho) nullval * emp))) 
-=
-@Sep.sexprD all_types (functions ++ (more_funcs rho contents sh))  
-predicates nil nil (left_side)).
-simpl.
-unfold VericSepLogic.star.
-unfold VericSepLogic.inj.
-unfold VericSepLogic.emp.
-(*close, but not exactly equal because of emp in reified version*)
+prepare_reify.
+
+replace
+(!!(True /\
+      eval_id _t rho = eval_id _p rho /\
+      eval_id _s rho = Vint (Int.repr 0) /\ True) && emp *
+   (lseg LS sh (map Vint contents) (eval_id _p rho) nullval * emp))
+with
+(@Sep.sexprD all_types (functions ++ (more_funcs rho contents sh))  
+predicates nil nil (left_side)) by reflexivity.
+
+replace
+(!!(True /\
+          Vint (Int.sub (sum_int contents) (sum_int contents)) =
+          eval_id _s rho /\ True) && emp *
+       (!!True * lseg LS sh (map Vint contents) (eval_id _t rho) nullval * emp))
+with
+(@Sep.sexprD all_types (functions ++ (more_funcs rho contents sh))
+predicates nil nil (right_side)) by reflexivity.
+
+replace 
+(tc_environ Delta rho) with 
+(force_Opt (@Expr.exprD all_types (functions ++ (more_funcs rho contents sh)) nil nil tc_environ_r Expr.tvProp)False) in H3 by reflexivity.
+finish_reify.
+
 Admitted.
