reify/sep.v
@@ -3,7 +3,7 @@ Require Import floyd.proofauto.
 
 Local Open Scope logic.
 
-Module VericSepLogic <: SepTheory.SepTheory.
+Module VericSepLogic_Kernel <: SepTheory.SepTheory_Kernel.
 
 Definition hprop := mpred.
 Definition himp := derives.
@@ -11,39 +11,7 @@ Definition heq := fun p1 p2 => derives p1 p2 /\ derives p2 p1.
 Definition Refl_himp := derives_refl.
 Definition Trans_himp := derives_trans.
 
-Lemma Refl_heq : Reflexive heq.
-Proof. 
-intros. 
-unfold heq; split; apply derives_refl; auto.
-Qed.
-
-Lemma Sym_heq : Symmetric heq.
-Proof.
-unfold heq, Symmetric. intros. intuition.
-Qed.
-
-Lemma Trans_heq : Transitive heq.
-Proof.
-unfold heq, Transitive; intros.
-intuition; eapply derives_trans; eauto.
-Qed.
-
-Local Notation "a ===> b" := (himp a b) (at level 60).
-Local Notation "a <===> b" := (heq a b) (at level 60).
-
-
-Lemma heq_defn : forall a b, (a ===> b /\ b ===> a) <-> a <===> b.
-Proof.
-intros. unfold heq, himp; intuition.
-Qed.
-
-Lemma heq_himp : forall a b, a <===> b -> a ===> b.
-Proof. intros.
-unfold heq, himp in *; intuition.
-Qed.
-
 Definition emp := emp.
-
 
 Definition inj := fun p => (prop p && emp).
 
@@ -51,88 +19,40 @@ Definition star := sepcon.
 
 Definition ex := @exp mpred Nveric. 
 
-Lemma himp_star_comm : forall P Q, 
-    (star P Q) ===> (star Q P).
-Proof.
-intros. unfold star, himp. cancel. 
-Qed.
-
-Lemma heq_star_comm : forall P Q, 
-    (star P Q) <===> (star Q P).
-Proof.
-intros. split; unfold star; cancel.
-Qed.
-
-Lemma heq_star_assoc : forall P Q R, 
-  (star (star P Q) R) <===> (star P (star Q R)).
-Proof.
-split; unfold star; cancel.
-Qed.
-
-Lemma heq_star_emp_l : forall P, (star emp P) <===> P.
-Proof.
-split; unfold star; cancel.
-Qed.
-
-Lemma heq_star_emp_r : forall P, (star P emp) <===> P.
-Proof.
-split; unfold star; cancel.
-Qed.
-
-Lemma himp_star_frame : forall P Q R S, 
-  P ===> Q -> R ===> S -> (star P R) ===> (star Q S).
-Proof.
-intros. unfold star. unfold himp in *. apply sepcon_derives; auto.
-Qed.
+Local Notation "a ===> b" := (himp a b) (at level 60).
 
 Ltac sep_solve :=
   unfold star, himp, heq, emp, inj, ex in *; intuition; cancel; auto.
 
-Lemma heq_star_frame : forall P Q R S, 
-  P <===> Q -> R <===> S -> (star P R) <===> (star Q S).
-Proof.
-intros; sep_solve.
-Qed.
 
-Lemma himp_subst_p : forall P Q R S,
-  P ===> S -> (star S Q) ===> R ->
-  (star P Q) ===> R.
-Proof.
-sep_solve.
-eapply derives_trans in H0. apply H0. cancel.
-Qed.
-
-Lemma himp_subst_c : forall P Q R S,
-  S ===> Q -> P ===> (star S R) ->
-  P ===> (star Q R).
-Proof.
-sep_solve.
-eapply derives_trans; eauto; cancel.
-Qed.
-
-Lemma heq_subst : forall P Q R S,
-  P <===> S -> (star S Q) <===> R ->
-  (star P Q) <===> R.
-Proof.
-sep_solve.
-eapply derives_trans in H; eauto; cancel.
-eapply derives_trans; eauto; cancel.
-Qed.
-
-Lemma himp_star_cancel : forall P Q R,
-  Q ===> R -> (star P Q) ===> (star P R).
+Lemma himp_star_comm : forall P Q, 
+    (star P Q) ===> (star Q P).
 Proof.
 sep_solve.
 Qed.
 
-Lemma heq_star_cancel : forall P Q R, 
-  Q <===> R -> (star P Q) <===> (star P R).
+Lemma himp_star_assoc : forall P Q R, 
+    (star (star P Q) R) ===> (star P (star Q R)).
 Proof.
 sep_solve.
 Qed.
 
+Lemma himp_star_emp_p : forall P, (star emp P) ===> P.
+Proof.
+sep_solve.
+Qed.
 
-(** pure lemmas **)
+Lemma himp_star_emp_c : forall P, P ===> (star emp P).
+Proof.
+sep_solve.
+Qed. 
+
+Lemma himp_star_frame : forall P Q R S, 
+  P ===> Q -> R ===> S -> (star P R) ===> (star Q S).
+Proof.
+sep_solve.
+Qed.
+
 Lemma himp_star_pure_p : forall P Q F,
   (star (inj F) P) ===> Q -> (F -> P ===> Q).
 Proof.
@@ -147,7 +67,7 @@ intros.
 sep_solve. entailer!.
 Qed.
 
-  Lemma himp_star_pure_cc : forall P Q (p : Prop),
+Lemma himp_star_pure_cc : forall P Q (p : Prop),
     p ->
     P ===> Q ->
     P ===> (star (inj p) Q).
@@ -155,7 +75,6 @@ Proof.
 sep_solve. entailer!.
 Qed.
 
-  (** ex lemmas **)
   Lemma himp_ex_p : forall T (P : T -> _) Q, 
             (forall v, (P v) ===> Q) -> (ex T P) ===> Q.
   Proof. sep_solve. apply exp_left. auto.
@@ -167,36 +86,23 @@ Qed.
  sep_solve. destruct H. eapply exp_right.  apply H.
 Qed.
 
-  Lemma heq_ex : forall T (P Q : T -> _), 
-    (forall v, P v <===> Q v) ->
-    ex T P <===> ex T Q.
-Proof. 
-sep_solve; apply exp_left;  intros;
-specialize (H x); destruct H; apply (exp_right x);
-auto.
-Qed.
-
-  Lemma himp_ex : forall T (P Q : T -> _), 
-    (forall v, P v ===> Q v) ->
-    ex T P ===> ex T Q.
-Proof.
-sep_solve. apply exp_left. intros.
-specialize (H x). apply (exp_right x). auto.
-Qed.
-
-  Lemma heq_ex_star : forall T (P : T -> _) Q,
-    (star (ex T P) Q) <===> (ex T (fun x => star (P x) Q)).
-Proof.
-sep_solve. entailer!.
-entailer!. apply (exp_right x). auto.
-Qed.
-
   Lemma himp_ex_star : forall T (P : T -> _) Q,
     (star (ex T P) Q) ===> (ex T (fun x => star (P x) Q)).
 Proof.
 sep_solve. entailer!.
 Qed.
 
-End VericSepLogic.
+Lemma himp_star_ex : forall T (P : T -> _) Q,
+     (ex T (fun x => star (P x) Q)) ===> (star (ex T P) Q).
+Proof.
+sep_solve.
+entailer!.
+apply (exp_right x).
+cancel.
+Qed. 
+
+End VericSepLogic_Kernel.
+
+Module VericSepLogic := SepTheory.SepTheory_From_Kernel VericSepLogic_Kernel.
 
 Module Sep := SepExpr.Make VericSepLogic.
